src/3d/Deps.fst
@@ -150,8 +150,8 @@ let scan_deps (fn:string) : ML scan_deps_t =
     match a.v with
     | Probe_atomic_action a -> deps_of_probe_atomic_action a
     | Probe_action_var e -> deps_of_expr e
-    | Probe_action_seq hd tl -> (deps_of_probe_action hd)@(deps_of_probe_action tl)
-    | Probe_action_let i a k -> (deps_of_probe_atomic_action a)@(deps_of_probe_action k)
+    | Probe_action_seq _ hd tl -> (deps_of_probe_action hd)@(deps_of_probe_action tl)
+    | Probe_action_let _ i a k -> (deps_of_probe_atomic_action a)@(deps_of_probe_action k)
     | Probe_action_ite e th el -> deps_of_expr e @ deps_of_probe_action th @ deps_of_probe_action el
     | Probe_action_array len b -> deps_of_expr len @ deps_of_probe_action b
   in
