src/3d/Simplify.fst
@@ -135,10 +135,10 @@ let rec simplify_probe_action (env:T.env_t) (a:probe_action) : ML probe_action =
   | Probe_action_var i -> a
   | Probe_atomic_action aa ->
     {a with v = Probe_atomic_action (simplify_probe_atomic_action env aa)}
-  | Probe_action_seq hd tl ->
-    {a with v = Probe_action_seq (simplify_probe_action env hd) (simplify_probe_action env tl) }
-  | Probe_action_let i aa k ->
-    {a with v = Probe_action_let i (simplify_probe_atomic_action env aa) (simplify_probe_action env k) }
+  | Probe_action_seq d hd tl ->
+    {a with v = Probe_action_seq d (simplify_probe_action env hd) (simplify_probe_action env tl) }
+  | Probe_action_let d i aa k ->
+    {a with v = Probe_action_let d i (simplify_probe_atomic_action env aa) (simplify_probe_action env k) }
   | Probe_action_ite hd then_ else_ ->
     {a with v = Probe_action_ite (simplify_expr env hd) (simplify_probe_action env then_)
                                  (simplify_probe_action env else_) }
