src/3d/Target.fst
@@ -617,10 +617,10 @@ let rec print_probe_action (mname:string) (p:probe_action) : ML string =
     Printf.sprintf "(Probe_action_atomic %s)" (print_atomic_probe_action a)
   | Probe_action_var e ->
     Printf.sprintf "(Probe_action_var %s)" (print_expr mname e)
-  | Probe_action_seq p1 p2 ->
-    Printf.sprintf "(Probe_action_seq %s %s)" (print_probe_action mname p1) (print_probe_action mname p2)
-  | Probe_action_let i m1 m2 ->
-    Printf.sprintf "(Probe_action_let %s (fun %s -> %s))" (print_atomic_probe_action m1) (print_ident i) (print_probe_action mname m2)
+  | Probe_action_seq d p1 p2 ->
+    Printf.sprintf "(Probe_action_seq \"%s\" %s %s)" d (print_probe_action mname p1) (print_probe_action mname p2)
+  | Probe_action_let d i m1 m2 ->
+    Printf.sprintf "(Probe_action_let \"%s\" %s (fun %s -> %s))" d (print_atomic_probe_action m1) (print_ident i) (print_probe_action mname m2)
   | Probe_action_ite cond m1 m2 ->
     Printf.sprintf "(Probe_action_ite %s %s %s)" (print_expr mname cond) (print_probe_action mname m1) (print_probe_action mname m2)
   | Probe_action_array len b ->
